Move definitions

theories/Algorithmic/Typing/Definitions.v
@@ -8,7 +8,6 @@ Import Domain_Notations.
 
 Reserved Notation "Γ '⊢a' M ⟹ A" (in custom judg at level 80, Γ custom exp, M custom exp, A custom nf).
 Reserved Notation "Γ '⊢a' M ⟸ A" (in custom judg at level 80, Γ custom exp, M custom exp, A custom exp).
-(* Reserved Notation "Γ '⊢a' A @ i" (in custom judg at level 80, Γ custom exp, A custom exp, i constr). *)
 
 Generalizable All Variables.
 
@@ -55,51 +54,11 @@ with alg_type_infer : ctx -> nf -> exp -> Prop :=
      {{ Γ ⊢a #x ⟹ B }} )
 where "Γ '⊢a' M ⟹ A" := (alg_type_infer Γ A M) (in custom judg) : type_scope.
 
-(* Variant alg_univ_infer : ctx -> nat -> typ -> Prop := *)
-(* | aui_ati : *)
-(*   `( {{ Γ ⊢a A ⟹ Type@i }} -> *)
-(*      {{ Γ ⊢a A @ i }} ) *)
-(* where "Γ '⊢a' A @ i" := (alg_univ_infer Γ i A) (in custom judg) : type_scope. *)
-
 #[export]
-Hint Constructors alg_type_check alg_type_infer (* alg_univ_infer *) : mcltt.
+Hint Constructors alg_type_check alg_type_infer : mcltt.
 
 Scheme alg_type_check_mut_ind := Induction for alg_type_check Sort Prop
 with alg_type_infer_mut_ind := Induction for alg_type_infer Sort Prop.
 Combined Scheme alg_type_mut_ind from
   alg_type_check_mut_ind,
   alg_type_infer_mut_ind.
-
-Inductive user_exp : exp -> Prop :=
-| user_exp_typ :
-  `( user_exp {{{ Type@i }}} )
-| user_exp_nat :
-  `( user_exp {{{ ℕ }}} )
-| user_exp_zero :
-  `( user_exp {{{ zero }}} )
-| user_exp_succ :
-  `( user_exp {{{ M }}} ->
-     user_exp {{{ succ M }}} )
-| user_exp_natrec :
-  `( user_exp {{{ A }}} ->
-     user_exp {{{ MZ }}} ->
-     user_exp {{{ MS }}} ->
-     user_exp {{{ M }}} ->
-     user_exp {{{ rec M return A | zero -> MZ | succ -> MS end }}} )
-| user_exp_pi :
-  `( user_exp {{{ A }}} ->
-     user_exp {{{ B }}} ->
-     user_exp {{{ Π A B }}} )
-| user_exp_fn :
-  `( user_exp {{{ A }}} ->
-     user_exp {{{ M }}} ->
-     user_exp {{{ λ A M }}} )
-| user_exp_app :
-  `( user_exp {{{ M }}} ->
-     user_exp {{{ N }}} ->
-     user_exp {{{ M N }}} )
-| user_exp_vlookup :
-  `( user_exp {{{ #x }}} ).
-
-#[export]
-Hint Constructors user_exp : mcltt.
